progress

plf/References.v
@@ -132,3 +132,604 @@ Hint Unfold z : core.
 Definition tseq t1 t2 :=
   <{ (\ x : Unit, t2) t1 }>.
 Notation "t1 ; t2" := (tseq t1 t2) (in custom stlc at level 3).
+
+Definition store := list tm.
+
+Definition store_lookup (n:nat) (st:store) :=
+  nth n st <{ unit }>.
+
+Fixpoint replace {A:Type} (n:nat) (x:A) (l:list A) : list A :=
+    match l with
+    | nil => nil
+    | h :: t =>
+      match n with
+      | O => x :: t
+      | S n' => h :: replace n' x t
+      end
+    end.
+    
+Lemma replace_nil : forall A n (x:A),
+  replace n x nil = nil.
+Proof.
+  destruct n; auto.
+Qed.
+  
+Lemma length_replace : forall A n x (l:list A),
+  length (replace n x l) = length l.
+Proof with auto.
+  intros A n x l. generalize dependent n.
+  induction l; intros n.
+    destruct n...
+    destruct n...
+      simpl. rewrite IHl...
+Qed.
+  
+Lemma lookup_replace_eq : forall l t st,
+  l < length st ->
+  store_lookup l (replace l t st) = t.
+Proof with auto.
+  intros l t st.
+  unfold store_lookup.
+  generalize dependent l.
+  induction st as [|t' st']; intros l Hlen.
+  - (* st =  *)
+   inversion Hlen.
+  - (* st = t' :: st' *)
+    destruct l; simpl...
+    apply IHst'. simpl in Hlen. lia.
+Qed.
+
+Lemma lookup_replace_neq : forall l1 l2 t st,
+  l1 <> l2 ->
+  store_lookup l1 (replace l2 t st) = store_lookup l1 st.
+Proof with auto.
+  unfold store_lookup.
+  induction l1 as [|l1']; intros l2 t st Hneq.
+  - (* l1 = 0 *)
+    destruct st.
+    + (* st =  *) rewrite replace_nil...
+    + (* st = _ :: _ *) destruct l2... contradict Hneq...
+  - (* l1 = S l1' *)
+    destruct st as [|t2 st2].
+    + (* st =  *) destruct l2...
+    + (* st = t2 :: st2 *)
+      destruct l2...
+      simpl; apply IHl1'...
+Qed.
+
+Inductive step : tm * store -> tm * store -> Prop :=
+  | ST_AppAbs : forall x T2 t1 v2 st,
+         value v2 ->
+         <{ (\x : T2, t1) v2 }> / st --> <{ [x := v2] t1 }> / st
+  | ST_App1 : forall t1 t1' t2 st st',
+         t1 / st --> t1' / st' ->
+         <{ t1 t2 }> / st --> <{ t1' t2 }> / st'
+  | ST_App2 : forall v1 t2 t2' st st',
+         value v1 ->
+         t2 / st --> t2' / st' ->
+         <{ v1 t2 }> / st --> <{ v1 t2' }> / st'
+  (* numbers *)
+  | ST_SuccNat : forall (n : nat) st,
+         <{ succ n }> / st --> tm_const (S n) / st
+  | ST_Succ : forall t1 t1' st st',
+         t1 / st --> t1' / st' ->
+         <{ succ t1 }> / st --> <{ succ t1' }> / st'
+  | ST_PredNat : forall (n : nat) st,
+         <{ pred n }> / st --> tm_const (n - 1) / st
+  | ST_Pred : forall t1 t1' st st',
+         t1 / st --> t1' / st' ->
+         <{ pred t1 }> / st --> <{ pred t1' }> / st'
+  | ST_MultNats : forall (n1 n2 : nat) st,
+      <{ n1 * n2 }> / st --> tm_const (n1 * n2) / st
+  | ST_Mult1 : forall t1 t2 t1' st st',
+         t1 / st --> t1' / st' ->
+         <{ t1 * t2 }> / st --> <{ t1' * t2 }> / st'
+  | ST_Mult2 : forall v1 t2 t2' st st',
+         value v1 ->
+         t2 / st --> t2' / st' ->
+         <{ v1 * t2 }> / st --> <{ v1 * t2' }> / st'
+  | ST_If0 : forall t1 t1' t2 t3 st st',
+         t1 / st --> t1' / st' ->
+         <{ if0 t1 then t2 else t3 }> / st --> <{ if0 t1' then t2 else t3 }> / st'
+  | ST_If0_Zero : forall t2 t3 st,
+         <{ if0 0 then t2 else t3 }> / st --> t2 / st
+  | ST_If0_Nonzero : forall n t2 t3 st,
+         <{ if0 {S n} then t2 else t3 }> / st --> t3 / st
+  (* references *)
+  | ST_RefValue : forall v st,
+         value v ->
+         <{ ref v }> / st --> <{ loc { length st } }> / (st ++ v::nil)
+  | ST_Ref : forall t1 t1' st st',
+         t1 / st --> t1' / st' ->
+         <{ ref t1 }> / st --> <{ ref t1' }> / st'
+  | ST_DerefLoc : forall st l,
+         l < length st ->
+         <{ !(loc l) }> / st --> <{ { store_lookup l st } }> / st
+  | ST_Deref : forall t1 t1' st st',
+         t1 / st --> t1' / st' ->
+         <{ ! t1 }> / st --> <{ ! t1' }> / st'
+  | ST_Assign : forall v l st,
+         value v ->
+         l < length st ->
+         <{ (loc l) := v }> / st --> <{ unit }> / replace l v st
+  | ST_Assign1 : forall t1 t1' t2 st st',
+         t1 / st --> t1' / st' ->
+         <{ t1 := t2 }> / st --> <{ t1' := t2 }> / st'
+  | ST_Assign2 : forall v1 t2 t2' st st',
+         value v1 ->
+         t2 / st --> t2' / st' ->
+         <{ v1 := t2 }> / st --> <{ v1 := t2' }> / st'
+
+where "t '/' st '-->' t' '/' st'" := (step (t,st) (t',st')).
+
+Hint Constructors step : core.
+Definition multistep := (multi step).
+Notation "t '/' st '-->*' t' '/' st'" :=
+               (multistep (t,st) (t',st'))
+               (at level 40, st at level 39, t' at level 39).
+               
+Definition context := partial_map ty.
+
+Theorem cyclic_store:
+  exists t,
+    t / nil -->*
+    <{ unit }> / (<{ \x:Nat, (!(loc 1)) x }> :: <{ \x:Nat, (!(loc 0)) x }> :: nil).
+Proof.
+  exists 
+  <{ ref 0; ref 0; 
+    (loc 0 := \x:Nat, (!(loc 1)) x);
+    (loc 1 := \x:Nat, (!(loc 0)) x)
+  }>.
+  unfold ";".
+Admitted.
+
+Definition store_ty := list ty.
+
+Definition store_Tlookup (n:nat) (ST:store_ty) :=
+  nth n ST <{ Unit }>.
+
+Reserved Notation "Gamma ';' ST '|--' t '\in' T"
+                  (at level 40, t custom stlc, T custom stlc at level 0).
+                  
+Inductive has_type (ST : store_ty) : context -> tm -> ty -> Prop :=
+| T_Var : forall Gamma x T1,
+    Gamma x = Some T1 ->
+    Gamma ; ST |-- x \in T1
+| T_Abs : forall Gamma x T1 T2 t1,
+    update Gamma x T2 ; ST |-- t1 \in T1 ->
+    Gamma ; ST |-- \x:T2, t1 \in (T2 -> T1)
+| T_App : forall T1 T2 Gamma t1 t2,
+    Gamma ; ST |-- t1 \in (T2 -> T1) ->
+    Gamma ; ST |-- t2 \in T2 ->
+    Gamma ; ST |-- t1 t2 \in T1
+| T_Nat : forall Gamma (n : nat),
+    Gamma ; ST |-- n \in Nat
+| T_Succ : forall Gamma t1,
+    Gamma ; ST |-- t1 \in Nat ->
+    Gamma ; ST |-- succ t1 \in Nat
+| T_Pred : forall Gamma t1,
+    Gamma ; ST |-- t1 \in Nat ->
+    Gamma ; ST |-- pred t1 \in Nat
+| T_Mult : forall Gamma t1 t2,
+    Gamma ; ST |-- t1 \in Nat ->
+    Gamma ; ST |-- t2 \in Nat ->
+    Gamma ; ST |-- t1 * t2 \in Nat
+| T_If0 : forall Gamma t1 t2 t3 T0,
+    Gamma ; ST |-- t1 \in Nat ->
+    Gamma ; ST |-- t2 \in T0 ->
+    Gamma ; ST |-- t3 \in T0 ->
+    Gamma ; ST |-- if0 t1 then t2 else t3 \in T0
+| T_Unit : forall Gamma,
+    Gamma ; ST |-- unit \in Unit
+| T_Loc : forall Gamma l,
+    l < length ST ->
+    Gamma ; ST |-- (loc l) \in (Ref {store_Tlookup l ST })
+| T_Ref : forall Gamma t1 T1,
+    Gamma ; ST |-- t1 \in T1 ->
+    Gamma ; ST |-- (ref t1) \in (Ref T1)
+| T_Deref : forall Gamma t1 T1,
+    Gamma ; ST |-- t1 \in (Ref T1) ->
+    Gamma ; ST |-- (! t1) \in T1
+| T_Assign : forall Gamma t1 t2 T2,
+    Gamma ; ST |-- t1 \in (Ref T2) ->
+    Gamma ; ST |-- t2 \in T2 ->
+    Gamma ; ST |-- (t1 := t2) \in Unit
+where "Gamma ';' ST '|--' t '\in' T" := (has_type ST Gamma t T).
+
+Hint Constructors has_type : core.
+
+Theorem preservation_wrong1 : forall ST T t st t' st',
+  empty ; ST |-- t \in T ->
+  t / st --> t' / st' ->
+  empty ; ST |-- t' \in T.
+Abort.
+
+Definition store_well_typed (ST:store_ty) (st:store) :=
+  length ST = length st /\
+  (forall l, l < length st ->
+     empty; ST |-- { store_lookup l st } \in {store_Tlookup l ST }).
+     
+Theorem store_not_unique:
+  exists st, exists ST1, exists ST2,
+    store_well_typed ST1 st /\
+    store_well_typed ST2 st /\
+    ST1 <> ST2.
+Proof.
+  exists (<{!(loc 0)}> :: nil), (Ty_Nat :: nil), (Ty_Unit :: nil).
+  
+  (* FILL IN HERE *) Admitted.
+
+Theorem preservation_wrong2 : forall ST T t st t' st',
+  empty ; ST |-- t \in T ->
+  t / st --> t' / st' ->
+  store_well_typed ST st ->
+  empty ; ST |-- t' \in T.
+Abort.
+
+Inductive extends : store_ty -> store_ty -> Prop :=
+  | extends_nil : forall ST',
+      extends ST' nil
+  | extends_cons : forall x ST' ST,
+      extends ST' ST ->
+      extends (x::ST') (x::ST).
+Hint Constructors extends : core.
+
+Lemma extends_lookup : forall l ST ST',
+  l < length ST ->
+  extends ST' ST ->
+  store_Tlookup l ST' = store_Tlookup l ST.
+Proof with auto.
+  intros l ST.
+  generalize dependent l.
+  induction ST as [|a ST2]; intros l ST' Hlen HST'.
+  - (* nil *) inversion Hlen.
+  - (* cons *) unfold store_Tlookup in *.
+    destruct ST'.
+    + (* ST' = nil *) inversion HST'.
+    + (* ST' = a' :: ST'2 *)
+      inversion HST'; subst.
+      destruct l as [|l'].
+      * (* l = 0 *) auto.
+      * (* l = S l' *) simpl. apply IHST2...
+        simpl in Hlen; lia.
+Qed.
+
+Lemma length_extends : forall l ST ST',
+  l < length ST ->
+  extends ST' ST ->
+  l < length ST'.
+Proof with eauto.
+  intros. generalize dependent l. induction H0; intros l Hlen.
+    - inversion Hlen.
+    - simpl in *.
+      destruct l; try lia.
+        apply ->Nat.succ_lt_mono. apply IHextends. lia.
+Qed.
+
+Lemma extends_app : forall ST T,
+  extends (ST ++ T) ST.
+Proof.
+  induction ST; intros T.
+  auto.
+  simpl. auto.
+Qed.
+
+Lemma extends_refl : forall ST,
+  extends ST ST.
+Proof.
+  induction ST; auto.
+Qed.
+
+Definition preservation_theorem := forall ST t t' T st st',
+  empty ; ST |-- t \in T ->
+  store_well_typed ST st ->
+  t / st --> t' / st' ->
+  exists ST',
+     extends ST' ST /\
+     empty ; ST' |-- t' \in T /\
+     store_well_typed ST' st'.
+     
+     Lemma weakening : forall Gamma Gamma' ST t T,
+     includedin Gamma Gamma' ->
+     Gamma ; ST |-- t \in T ->
+     Gamma' ; ST |-- t \in T.
+Proof.
+  intros Gamma Gamma' ST t T H Ht.
+  generalize dependent Gamma'.
+  induction Ht; eauto using includedin_update.
+Qed.
+
+Lemma weakening_empty : forall Gamma ST t T,
+     empty ; ST |-- t \in T ->
+     Gamma ; ST |-- t \in T.
+Proof.
+  intros Gamma ST t T.
+  eapply weakening.
+  discriminate.
+Qed.
+
+Lemma substitution_preserves_typing : forall Gamma ST x U t v T,
+  (update Gamma x U); ST |-- t \in T ->
+  empty ; ST |-- v \in U ->
+  Gamma ; ST |-- [x:=v]t \in T.
+Proof.
+  intros Gamma ST x U t v T Ht Hv.
+  generalize dependent Gamma. generalize dependent T.
+  induction t; intros T Gamma H;
+  (* in each case, we'll want to get at the derivation of H *)
+    inversion H; clear H; subst; simpl; eauto.
+  - (* var *)
+    rename s into y. destruct (String.eqb_spec x y); subst.
+    + (* x=y *)
+      rewrite update_eq in H2.
+      injection H2 as H2; subst.
+      apply weakening_empty. assumption.
+    + (* x<>y *)
+      apply T_Var. rewrite update_neq in H2; auto.
+  - (* abs *)
+    rename s into y.
+    destruct (String.eqb_spec x y); subst; apply T_Abs.
+    + (* x=y *)
+      rewrite update_shadow in H5. assumption.
+    + (* x<>y *)
+      apply IHt.
+      rewrite update_permute; auto.
+Qed.
+
+Lemma assign_pres_store_typing : forall ST st l t,
+  l < length st ->
+  store_well_typed ST st ->
+  empty ; ST |-- t \in {store_Tlookup l ST} ->
+  store_well_typed ST (replace l t st).
+Proof with auto.
+  intros ST st l t Hlen HST Ht.
+  inversion HST; subst.
+  split. rewrite length_replace...
+  intros l' Hl'.
+  destruct (l' =? l) eqn: Heqll'.
+  - (* l' = l *)
+    apply eqb_eq in Heqll'; subst.
+    rewrite lookup_replace_eq...
+  - (* l' <> l *)
+    apply eqb_neq in Heqll'.
+    rewrite lookup_replace_neq...
+    rewrite length_replace in Hl'.
+    apply H0...
+Qed.
+
+Lemma store_weakening : forall Gamma ST ST' t T,
+  extends ST' ST ->
+  Gamma ; ST |-- t \in T ->
+  Gamma ; ST' |-- t \in T.
+Proof with eauto.
+  intros. induction H0; eauto.
+  - (* T_Loc *)
+    rewrite <- (extends_lookup _ _ ST')...
+    apply T_Loc.
+    eapply length_extends...
+Qed.
+
+Lemma store_well_typed_app : forall ST st t1 T1,
+  store_well_typed ST st ->
+  empty ; ST |-- t1 \in T1 ->
+  store_well_typed (ST ++ T1::nil) (st ++ t1::nil).
+Proof with auto.
+  intros.
+  unfold store_well_typed in *.
+  destruct H as [Hlen Hmatch].
+  rewrite app_length, add_comm. simpl.
+  rewrite app_length, add_comm. simpl.
+  split...
+  - (* types match. *)
+    intros l Hl.
+    unfold store_lookup, store_Tlookup.
+    apply le_lt_eq_dec in Hl; destruct Hl as [Hlt | Heq].
+    + (* l < length st *)
+      apply <-Nat.succ_lt_mono in Hlt.
+      rewrite !app_nth1...
+      * apply store_weakening with ST. apply extends_app.
+        apply Hmatch...
+      * rewrite Hlen...
+    + (* l = length st *)
+      injection Heq as Heq; subst.
+      rewrite app_nth2; try lia.
+      rewrite <- Hlen.
+      rewrite sub_diag. simpl.
+      apply store_weakening with ST...
+      { apply extends_app. }
+      rewrite app_nth2; [|lia].
+      rewrite sub_diag. simpl. assumption.
+Qed.
+
+Lemma nth_eq_last : forall A (l:list A) x d,
+  nth (length l) (l ++ x::nil) d = x.
+Proof.
+  induction l; intros; [ auto | simpl; rewrite IHl; auto ].
+Qed.
+
+Theorem preservation : forall ST t t' T st st',
+  empty ; ST |-- t \in T ->
+  store_well_typed ST st ->
+  t / st --> t' / st' ->
+  exists ST',
+     extends ST' ST /\
+     empty ; ST' |-- t' \in T /\
+     store_well_typed ST' st'.
+Proof with eauto using store_weakening, extends_refl.
+  remember empty as Gamma.
+  intros ST t t' T st st' Ht.
+  generalize dependent t'.
+  induction Ht; intros t' HST Hstep;
+    subst; try solve_by_invert; inversion Hstep; subst;
+    try (eauto using store_weakening, extends_refl).
+  (* T_App *)
+  - (* ST_AppAbs *) exists ST.
+    inversion Ht1; subst.
+    split; try split... eapply substitution_preserves_typing...
+  - (* ST_App1 *)
+    eapply IHHt1 in H0...
+    destruct H0 as [ST' [Hext [Hty Hsty]]].
+    exists ST'...
+  - (* ST_App2 *)
+    eapply IHHt2 in H5...
+    destruct H5 as [ST' [Hext [Hty Hsty]]].
+    exists ST'...
+  - (* T_Succ *)
+    + (* ST_Succ *)
+      eapply IHHt in H0...
+      destruct H0 as [ST' [Hext [Hty Hsty]]].
+      exists ST'...
+  - (* T_Pred *)
+    + (* ST_Pred *)
+      eapply IHHt in H0...
+      destruct H0 as [ST' [Hext [Hty Hsty]]].
+      exists ST'...
+  (* T_Mult *)
+  - (* ST_Mult1 *)
+    eapply IHHt1 in H0...
+    destruct H0 as [ST' [Hext [Hty Hsty]]].
+    exists ST'...
+  - (* ST_Mult2 *)
+    eapply IHHt2 in H5...
+    destruct H5 as [ST' [Hext [Hty Hsty]]].
+    exists ST'...
+  - (* T_If0 *)
+    + (* ST_If0_1 *)
+      eapply IHHt1 in H0...
+      destruct H0 as [ST' [Hext [Hty Hsty]]].
+      exists ST'. split...
+  (* T_Ref *)
+  - (* ST_RefValue *)
+    exists (ST ++ T1::nil).
+    inversion HST; subst.
+    split.
+    { apply extends_app. }
+    split.
+    { replace <{ Ref T1 }>
+        with <{ Ref {store_Tlookup (length st) (ST ++ T1::nil)} }>.
+      { apply T_Loc.
+        rewrite <- H. rewrite app_length, add_comm. simpl. lia. }
+      unfold store_Tlookup. rewrite <- H. rewrite nth_eq_last.
+      reflexivity. }
+    apply store_well_typed_app; assumption.
+  - (* ST_Ref *)
+    eapply IHHt in H0...
+    destruct H0 as [ST' [Hext [Hty Hsty]]].
+    exists ST'...
+  (* T_Deref *)
+  - (* ST_DerefLoc *)
+    exists ST. split; try split...
+    destruct HST as [_ Hsty].
+    replace T1 with (store_Tlookup l ST).
+    apply Hsty...
+    inversion Ht; subst...
+  - (* ST_Deref *)
+    eapply IHHt in H0...
+    destruct H0 as [ST' [Hext [Hty Hsty]]].
+    exists ST'...
+  (* T_Assign *)
+  - (* ST_Assign *)
+    exists ST. split; try split...
+    eapply assign_pres_store_typing...
+    inversion Ht1; subst...
+  - (* ST_Assign1 *)
+    eapply IHHt1 in H0...
+    destruct H0 as [ST' [Hext [Hty Hsty]]].
+    exists ST'...
+  - (* ST_Assign2 *)
+    eapply IHHt2 in H5...
+    destruct H5 as [ST' [Hext [Hty Hsty]]].
+    exists ST'...
+Qed.
+
+Theorem progress : forall ST t T st,
+  empty ; ST |-- t \in T ->
+  store_well_typed ST st ->
+  (value t \/ exists t' st', t / st --> t' / st').
+Proof with eauto.
+  intros ST t T st Ht HST. remember empty as Gamma.
+  induction Ht; subst; try solve_by_invert...
+  - (* T_App *)
+    right. destruct IHHt1 as [Ht1p | Ht1p]...
+    + (* t1 is a value *)
+      inversion Ht1p; subst; try solve_by_invert.
+      destruct IHHt2 as [Ht2p | Ht2p]...
+      * (* t2 steps *)
+        destruct Ht2p as [t2' [st' Hstep]].
+        exists <{ (\ x0 : T0, t0) t2' }>, st'...
+    + (* t1 steps *)
+      destruct Ht1p as [t1' [st' Hstep]].
+      exists <{ t1' t2 }>, st'...
+  - (* T_Succ *)
+    right. destruct IHHt as [Ht1p | Ht1p]...
+    + (* t1 is a value *)
+      inversion Ht1p; subst; try solve [ inversion Ht ].
+      * (* t1 is a const *)
+        exists <{ {S n} }>, st...
+    + (* t1 steps *)
+      destruct Ht1p as [t1' [st' Hstep]].
+      exists <{ succ t1' }>, st'...
+  - (* T_Pred *)
+    right. destruct IHHt as [Ht1p | Ht1p]...
+    + (* t1 is a value *)
+      inversion Ht1p; subst; try solve [inversion Ht ].
+      * (* t1 is a const *)
+        exists <{ {n - 1} }>, st...
+    + (* t1 steps *)
+      destruct Ht1p as [t1' [st' Hstep]].
+      exists <{ pred t1' }>, st'...
+  - (* T_Mult *)
+    right. destruct IHHt1 as [Ht1p | Ht1p]...
+    + (* t1 is a value *)
+      inversion Ht1p; subst; try solve [inversion Ht1].
+      destruct IHHt2 as [Ht2p | Ht2p]...
+      * (* t2 is a value *)
+        inversion Ht2p; subst; try solve [inversion Ht2].
+        exists <{ {n * n0} }>, st...
+      * (* t2 steps *)
+        destruct Ht2p as [t2' [st' Hstep]].
+        exists <{ n * t2' }>, st'...
+    + (* t1 steps *)
+      destruct Ht1p as [t1' [st' Hstep]].
+      exists <{ t1' * t2 }>, st'...
+  - (* T_If0 *)
+    right. destruct IHHt1 as [Ht1p | Ht1p]...
+    + (* t1 is a value *)
+      inversion Ht1p; subst; try solve [inversion Ht1].
+      destruct n.
+      * (* n = 0 *) exists t2, st...
+      * (* n = S n' *) exists t3, st...
+    + (* t1 steps *)
+      destruct Ht1p as [t1' [st' Hstep]].
+      exists <{ if0 t1' then t2 else t3 }>, st'...
+  - (* T_Ref *)
+    right. destruct IHHt as [Ht1p | Ht1p]...
+    + (* t1 steps *)
+      destruct Ht1p as [t1' [st' Hstep]].
+      exists <{ref t1'}>, st'...
+  - (* T_Deref *)
+    right. destruct IHHt as [Ht1p | Ht1p]...
+    + (* t1 is a value *)
+      inversion Ht1p; subst; try solve_by_invert.
+      eexists. eexists. apply ST_DerefLoc...
+      inversion Ht; subst. inversion HST; subst.
+      rewrite <- H...
+    + (* t1 steps *)
+      destruct Ht1p as [t1' [st' Hstep]].
+      exists <{ ! t1' }>, st'...
+  - (* T_Assign *)
+    right. destruct IHHt1 as [Ht1p|Ht1p]...
+    + (* t1 is a value *)
+      destruct IHHt2 as [Ht2p|Ht2p]...
+      * (* t2 is a value *)
+        inversion Ht1p; subst; try solve_by_invert.
+        eexists. eexists. apply ST_Assign...
+        inversion HST; subst. inversion Ht1; subst.
+        rewrite H in H4...
+      * (* t2 steps *)
+        destruct Ht2p as [t2' [st' Hstep]].
+        exists <{ t1 := t2' }>, st'...
+    + (* t1 steps *)
+      destruct Ht1p as [t1' [st' Hstep]].
+      exists <{ t1' := t2 }>, st'...
+Qed.
